Book: [[MATH2068]]
# Lemma 7.4
Let $(a_{jk})$ be a sequence of real numbers.
Suppose $\displaystyle \sum_{k=0}^{\infty}\sum_{j=0}^{k}\abs{a_{jk}}$ converges.
Then $\displaystyle \sum_{k=0}^{\infty}\sum_{j=0}^{k}a_{jk}$ converges to some $L$
Also, $\displaystyle \sum_{j=0}^{\infty}\sum_{k=j}^{\infty}a_{jk}$ converges to $L$.
#### Proof
Let $\varepsilon>0$.
Then $\exists K_{1}\in \mathbb{Z}_{>0}$ s.t. $\forall K\geq K_{1}:\displaystyle \abs*{L-\sum_{k=0}^{K}\sum_{j=0}^{k}a_{jk}}< \frac{\varepsilon}{2}$
Also, $\exists K_{2}\in \mathbb{Z}_{>0}$ s.t. $\displaystyle \sum_{k=K_{2}}^{\infty}\sum_{j=0}^{k}\abs{a_{jk}}< \frac{\varepsilon}{4}$ by cauchy criterion.
Take $J_{1}=\max\set{K_{1},K_{2}}$ and let $J\geq J_{1}$. Then
$$\begin{align}
\abs*{L-\sum_{j=0}^{J}\sum_{k=j}^{\infty}a_{jk}}&\leq \abs*{L-\sum_{j=0}^{J_{1}}\sum_{k=j}^{\infty}a_{jk}}+\abs*{\sum_{j=J_{1}}^{J}\sum_{k=j}^{\infty}a_{jk}} \\
&\leq \abs*{L-\sum_{j=0}^{J_{1}}\left( \sum_{k=j}^{J_{1}}a_{jk}+\sum_{k=J_{1}}^{\infty} a_{jk}\right)}+\sum_{j=J_{1}}^{J}\sum_{k=j}^{\infty}\abs{a_{jk}} \\
&\leq \abs*{L-\sum_{j=0}^{J_{1}} \sum_{k=j}^{J_{1}}a_{jk}}+\abs*{\sum_{j=0}^{J_{1}}\sum_{k=J_{1}}^{\infty}a_{jk}}+\sum_{j=J_{1}}^{J}\sum_{k=j}^{J}\abs{a_{jk}}+\sum_{j=J_{1}}^{J}\sum_{k=J}^{\infty}\abs{a_{jk}} \\
&\leq \abs*{L-\sum_{j=0}^{J_{1}} \sum_{k=j}^{J_{1}}a_{jk}}+\sum_{j=0}^{J_{1}}\sum_{k=J_{1}}^{\infty}\abs{a_{jk}}+\sum_{k=J_{1}}^{J}\sum_{j=J_{1}}^{k}\abs{a_{jk}}+\sum_{k=J}^{\infty}\sum_{j=J_{1}}^{J}\abs{a_{jk}} \\
&= \abs*{L-\sum_{k=0}^{J_{1}} \sum_{j=0}^{k}a_{jk}}+\sum_{k=J_{1}}^{\infty}\sum_{j=0}^{J_{1}}\abs{a_{jk}}+\sum_{k=J_{1}}^{\infty}\sum_{j=J_{1}}^{k}\abs{a_{jk}} \\
&= \abs*{L-\sum_{k=0}^{J_{1}} \sum_{j=0}^{k}a_{jk}}+\sum_{k=J_{1}}^{\infty}\sum_{j=0}^{k}\abs{a_{jk}}+\sum_{k=J_{1}}^{\infty}\sum_{j=J_{1}}^{k}\abs{a_{jk}} \\
&<\varepsilon
\end{align}$$

