Book: [[MATH2068]]
# Proposition 6.12 (Derivatives of power series)
Let $f=\sum a_{k}x^{k}$ be a power series with radius of convergence $r$.
If $r>0$ then $f\in C^{\infty}(-r,r)$ and $\forall x\in(-r,r)$, we have
$$f^{(k)}(x)=\sum_{n=k}^{\infty}\frac{a_{n}n!}{(n-k)!}x^{n-k}=\sum_{n=0}^{\infty} \frac{a_{n+k}(n+k)!}{n!}x^{n}$$
#### Proof
Let $c\in(-r,r)$. Then $\exists \eta\in(0,r)$ s.t. $f$ converges uniformly on $(-\eta,\eta)$
Consider $\sum (a_{n}x^{n})'=\sum a_{n}nx^{n-1}$.
Since $\lim\abs{na_{n}}^{1/n}=\lim\abs{a_{n}}^{1/n}$, $\sum a_{n}nx^{n-1}$ has radius of convergence $r$.
Now $\sum a_{n}nx^{n-1}$ converges uniformly on $(-\eta,\eta)$.
Hence $f|_{(-\eta,\eta)}$ is differentiable and all that shit
Now induction