Book: [[MATH2068]]
# Theorem 5.5 (Abs conv implies rearrangements abs conv)
Let $\sum a_{n}$ be abs conv.
Then any rearrangement $\sum a_{\sigma(n)}$ is abs conv.
Moreover, $\sum a_{\sigma(n)}=\sum a_{n}$.
#### Proof
Let $\sigma:\mathbb{Z}_{>0}\to \mathbb{Z}_{>0}$ be a bijection.
Let $\varepsilon>0$. 
Since $\sum\abs{a_{n}}<\infty$, $\exists N\in \mathbb{Z}_{>0}:\forall p\in \mathbb{Z}_{>0}:\displaystyle \sum_{k=1}^{p}\abs{a_{N+k}}<\varepsilon$.
Take $M=\max\sigma ^{-1}(\ii{1}{N})+1$. Then $i\geq M\implies\sigma(i)\geq N$.
Now $\forall i\geq M,p\in \mathbb{Z}_{>0}:\displaystyle \sum_{k=1}^{p}\abs{a_{\sigma(i+k)}}<\varepsilon$.
Hence $\sum a_{\sigma(n)}$ is abs conv by cauchy criterion.

Now denote $L=\sum a_{n},\ell=\sum a_{\sigma(n)}$
Let $\varepsilon>0$.
Since $L=\sum a_{n},$ $\exists N\in \mathbb{Z}_{>0}:\abs*{L-\displaystyle \sum_{i=1}^{N}a_{i}}<\varepsilon$ and $\forall p\in \mathbb{Z}_{>0}:\displaystyle \sum_{i=1}^{p}\abs{a_{N+i}}<\varepsilon$ by cauchy criterion.
Since $\ell=\sum a_{\sigma(n)}$, $\displaystyle \exists M\in \mathbb{Z}_{>0}:\abs*{\ell-\sum_{i=1}^{M}a_{\sigma(i)}}<\varepsilon$.
Take $M'=\max(\sigma ^{-1}(\ii{1}{N})\cup \set{M})$. Then $\ii{1}{N}\subseteq \set{\sigma(i)}_{i=1}^{M'}$.
Take $N'=\max(\set{\sigma(i)}_{i=1}^{M'})$.
Then $\displaystyle \abs*{\sum_{k=1}^{N}a_{n}-\sum_{i=1}^{M}a_{\sigma(i)}}\leq \sum_{i=N+1}^{N'}\abs{a_{i}}<\varepsilon$.
Hence $\abs{L-\ell}\leq \displaystyle \abs*{L-\sum_{i=1}^{N}a_{i}}+\abs*{\sum_{k=1}^{N}a_{n}-\sum_{i=1}^{M}a_{\sigma(i)}}+\abs*{\sum_{i=1}^{M}a_{\sigma(i)}-\ell}<3\varepsilon$.
#### Proof 2
Let $\sigma:\mathbb{Z}_{>0}\to \mathbb{Z}_{>0}$ be a bijection.
Let $\varepsilon>0$. 
Since $\sum\abs{a_{n}}<\infty$, $\exists N\in \mathbb{Z}_{>0}:\displaystyle \sum_{k=N}^{\infty}\abs{a_{k}}<\varepsilon$ and $\displaystyle \abs*{A-\sum_{k=1}^{n}a_{k}}<\varepsilon$ for all $n\geq N$.
Take $M=\max\sigma ^{-1}(\ii{1}{N})+1$. Then $i\geq M\implies\sigma(i)\geq N$.
Then $\ii{1}{N}\subseteq \sigma(\ii{1}{M})$ and $M\geq N$.
Thus $\forall n\geq M$,
$$\begin{align}
\abs*{A-\sum_{i=1}^{n}a_{\sigma(i)}}&\leq \abs*{A-\sum_{i=1}^{n}a_{i}}+\abs*{\sum_{i=1}^{n}a_{i}-\sum_{i=1}^{n}a_{\sigma(i)}} \\
&<\varepsilon+\abs*{\sum_{i=N+1}^{n}a_{i}-\sum_{j\in \sigma(\ii{1}{n})\setminus\ii{1}{N}}a_{j}} \\
&\leq\varepsilon+\abs*{\sum_{i=N+1}^{n}a_{i}}+\abs*{\sum_{j\in \sigma(\ii{1}{n})\setminus\ii{1}{N}}a_{j}} \\
&<3\varepsilon
\end{align}$$.
